some update; client03 WIP

src/example/Client03.v
@@ -27,12 +27,21 @@ Module Client03.
       _ <- (OMod.call (R:=unit) "store" (C, SCMem.val_add c n));;
       _ <- (trigger Yield;;; Spinlock.unlock L);; Ret tt.
 
+    Definition read :
+      itree (threadE ident state) SCMem.val
+      :=
+      _ <- (trigger Yield;;; Spinlock.lock L);;
+      c <- (OMod.call (R:=SCMem.val) "load" C);;
+      _ <- (trigger Yield;;; Spinlock.unlock L);;
+      Ret c.
+
     Definition thread1 :
       ktree (threadE ident state) unit SCMem.val
       :=
       fun _ =>
         _ <- trigger Yield;;
-        a <- Ret (0 : nat);;
+        let a := (0 : nat) in
+        (* a <- Ret (0 : nat);; *)
         _ <- (ITree.iter (fun (i : nat) =>
                            r <- (if (Nat.eq_dec i 100)
                                 then Ret (inr tt)
@@ -43,7 +52,7 @@ Module Client03.
                            b <- (OMod.call (R:=bool) "compare" (d, 0 : SCMem.val));;
                            r <- (if b
                                 then Ret (inl tt)
-                                else c <- (OMod.call (R:=SCMem.val) "load" C);; Ret (inr c));;
+                                else c <- read;; Ret (inr c));;
                            Ret r) tt);;
         _ <- trigger Yield;;
         Ret r.
@@ -53,14 +62,15 @@ Module Client03.
       :=
       fun _ =>
         _ <- trigger Yield;;
-        a <- Ret (0 : nat);;
+        let a := (0 : nat) in
+        (* a <- Ret (0 : nat);; *)
         _ <- (ITree.iter (fun (i : nat) =>
                            r <- (if (Nat.eq_dec i 10)
                                 then Ret (inr tt)
                                 else _ <- incr 5;; _ <- trigger Yield;; Ret (inl (i + 1)));;
                            Ret r) a);;
         _ <- (OMod.call (R:=unit) "store" (D, 1 : SCMem.val));;
-        r <- (OMod.call (R:=SCMem.val) "load" C);;
+        r <- read;;
         _ <- trigger Yield;;
         Ret r.
 
@@ -119,7 +129,6 @@ Section SPEC.
   Notation src_ident := (Mod.ident Client03Spec.module).
   Notation tgt_state := (Mod.state Client03.module).
   Notation tgt_ident := (Mod.ident Client03.module).
-  (* Notation tgt_ident := (void + SCMem.val)%type. *)
 
   Local Instance STT : StateTypes := Build_StateTypes src_state tgt_state src_ident tgt_ident.
   Context `{Σ : GRA.t}.
@@ -135,52 +144,135 @@ Section SPEC.
   Definition N_counter_inv : namespace := (N_Client03 .@ "counter").
   Definition N_t2_write_inv : namespace := (N_Client03 .@ "t2_write").
 
-  Definition counter r1 r2 n : Formula n :=
-    (∃ (x y : τ{nat}), (C ↦ ((2 * x) + (5 * y))) ∗ ➢(auexa_b r1 (x : nat)) ∗ ➢(auexa_b r2 (y : nat)))%F.
+  Definition counter n c1 c2 r1 r2 : Formula n :=
+    (∃ (x y : τ{nat}), (C ↦ ((c1 * x) + (c2 * y))) ∗ ➢(auexa_b r1 (x : nat)) ∗ ➢(auexa_b r2 (y : nat)))%F.
 
-  Definition counter_inv r1 r2 n : Formula n :=
-    (syn_inv n N_counter_inv (counter r1 r2 n)).
+  (* Definition counter_inv n r1 r2 : Formula n := *)
+  (*   (syn_inv n N_counter_inv (counter n r1 r2)). *)
 
-  Definition t2_write n : Formula n :=
-    (D ↦ 1)%F.
+  Definition t2_write n r : Formula n :=
+    (➢(auexa_w r (10 : nat)) ∗ (D ↦ 1))%F.
 
-  Definition t2_write_inv n : Formula n :=
-    (syn_inv n N_t2_write_inv (t2_write n))%F.
+  Definition t2_write_inv n r : Formula n :=
+    (syn_inv n N_t2_write_inv (t2_write n r))%F.
 
   (** Simulation proof. *)
 
-  Lemma Client03_thread1_spec
-        tid
+  Lemma Client03_incr_spec
+        tid N Es c1 c2
+        (TOP : OwnEs_top Es)
     :
-    ⊢ ⟦(∀ (r k w r1 r2 : τ{nat, 2}),
-           ((syn_tgt_interp_as 1 sndl (fun m => (➢ (scm_memory_black m))))
+    ⊢ ∀ (r k lft l r1 r2 a : τ{nat, 1+N}) (ds : list (nat * nat * Formula N)),
+        [@ tid, N, Es @]
+          ⧼⟦((syn_tgt_interp_as N sndl (λ m : SCMem.t, ➢(scm_memory_black m)))
+               ∗ (⤉ Duty(tid) ds) ∗ ◇{List.map fst ds}(lft, 1) ∗ ◇{List.map fst ds}(0, 1)
+               ∗ ◇{List.map fst ds}(0, 5)
+               ∗ (⤉ isSpinlock N r L (counter N c1 c2 r1 r2) k lft l)
+               ∗ (⌜2 <= l⌝) ∗ live[k] (1/2) ∗ ◇[k](1+l, 1)
+               ∗ ➢(auexa_w r1 (a : nat)))%F , 1+N⟧⧽
+            (OMod.close_itree omod (SCMem.mod gvs) (incr c1))
+            ⧼rv, ⟦((⤉ Duty(tid) ds) ∗ live[k] (1/2) ∗  ➢(auexa_w r1 (a + 1)))%F, 1+N⟧⧽
+  .
+  Proof.
+    iIntros. simpl. iStartTriple.
+    red_tl. simpl. rewrite red_syn_tgt_interp_as.
+    iIntros "(#MEM & DUTY & PCS_SPIN1 & PCS_SPIN2 & PCS & #ISL & %LE & LIVE_k & PC_k & CNTW_r1)".
+    iIntros "POST".
+    unfold incr. rred.
+    iMod (pcs_decr _ _ 4 1 with "PCS") as "[PCS PCS1]". auto.
+    iApply (wpsim_yieldR with "[DUTY PCS1]").
+    2:{ iFrame. }
+    auto.
+    iIntros "DUTY _". iModIntro. rred2r. iApply wpsim_tauR. rred2r.
+    iApply (Spinlock_lock_spec with "[LIVE_k DUTY PCS_SPIN1 PCS_SPIN2] [PCS PC_k CNTW_r1 POST]").
+    1,2: ss.
+    { red_tl. simpl. rewrite red_syn_tgt_interp_as. iSplit. eauto. iSplitR. eauto. iFrame. }
+    iEval (red_tl). iIntros (_) "[%u A]". iEval (unfold counter; red_tl) in "A".
+    iDestruct "A" as "([%x A] & LOCKED & LIVE_k & DUTY & LIVE_u & PC_u)". iEval (red_tl) in "A".
+    iDestruct "A" as "[%y A]". iEval (red_tl) in "A". iDestruct "A" as "(PT & CNTB_r1 & CNTB_r2)".
+    rred2r. iMod (pc_drop _ 1 _ _ 100 with "PC_u") as "PC_u". lia.
+    Unshelve. 2: lia.
+    iPoseProof (pc_split with "[PC_u]") as "[PC_u PC_u_pay]".
+    { iEval (replace 100 with (99 + 1)) in "PC_u". iFrame. }
+    iMod (pcs_decr _ _ 3 1 with "PCS") as "[PCS PCS1]". auto.
+    iApply (wpsim_yieldR with "[DUTY PC_u_pay PCS1]").
+    2:{ iSplitL "DUTY". iFrame. simpl. iApply pcs_cons_fold. iFrame. }
+    auto.
+    iIntros "DUTY _". iModIntro. rred2r.
+    iApply (SCMem_load_fun_spec with "[PT]").
+    3:{ iFrame. eauto. }
+    auto. ss.
+    iIntros (rv) "[%RV PT]". rred2r. iApply wpsim_tauR. rred2r.
+    iPoseProof (pc_split with "[PC_u]") as "[PC_u PC_u_pay]".
+    { iEval (replace 99 with (98 + 1)) in "PC_u". iFrame. }
+    iMod (pcs_decr _ _ 2 1 with "PCS") as "[PCS PCS1]". auto.
+    iApply (wpsim_yieldR with "[DUTY PC_u_pay PCS1]").
+    2:{ iSplitL "DUTY". iFrame. simpl. iApply pcs_cons_fold. iFrame. }
+    auto.
+    iIntros "DUTY _". iModIntro. rred2r.
+    iApply (SCMem_store_fun_spec with "[PT]").
+    3:{ iFrame. eauto. }
+    auto. ss.
+    iIntros (rv0) "PT". rred2r. iApply wpsim_tauR. rred2r.
+    iPoseProof (pc_split with "[PC_u]") as "[PC_u PC_u_pay]".
+    { iEval (replace 98 with (97 + 1)) in "PC_u". iFrame. }
+    iMod (pcs_decr _ _ 1 1 with "PCS") as "[PCS PCS1]". auto.
+    iApply (wpsim_yieldR with "[DUTY PC_u_pay PCS1]").
+    2:{ iSplitL "DUTY". iFrame. simpl. iApply pcs_cons_fold. iFrame. }
+    auto.
+    iIntros "DUTY _". iModIntro. rred2r. iApply wpsim_tauR. rred2r.
+    replace (SCMem.val_add rv c1) with ((c1 * (1 + x) + c2 * y) : SCMem.val).
+    2:{ subst rv. ss. f_equal. lia. }
+    iPoseProof (auexa_b_w_eq with "CNTB_r1 CNTW_r1") as "%EQ". subst a.
+    iMod (auexa_b_w_update _ _ _ _ nat (1 + x) with "CNTB_r1 CNTW_r1") as "[CNTB_r1 CNTW_r1]".
+    iApply (Spinlock_unlock_spec with "[CNTB_r1 CNTB_r2 PT LOCKED LIVE_k DUTY PCS LIVE_u PC_u PC_k]").
+    3:{ repeat (try rewrite @red_tl_sepconj). simpl.
+        iSplitR. rewrite red_syn_tgt_interp_as. eauto. iSplitR. eauto.
+        unfold counter. red_tl. iSplitL "PT CNTB_r1 CNTB_r2".
+        { iExists (1+x). red_tl. iExists y. red_tl. iFrame. }
+        Local Opaque progress_credits.
+        simpl. iEval (replace (l+1) with (S l) by lia). iFrame.
+        iApply pcs_cons_fold.
+        iPoseProof (pc_split with "[PC_u]") as "[PC1 PC2]". 2: iFrame.
+        simpl. replace 97 with (96 + 1) by ss. iFrame.
+        Local Transparent progress_credits.
+    }
+    ss. ss.
+    iEval red_tl. iIntros (_) "[DUTY LIVE_k]". rred2r.
+    iApply "POST". replace (1+x) with (x+1). iFrame. lia.
+  Qed.
+
+  Local Opaque incr.
+
+  Lemma Client03_thread1_spec
+        tid N
+    :
+    ⊢ ⟦(∀ (r k w r1 r2 : τ{nat, 1+N}),
+           ((syn_tgt_interp_as N sndl (fun m => (➢ (scm_memory_black m))))
                ∗ ○(tid)
                ∗ (⤉ Duty(tid) [])
-               ∗ (⤉ isSpinlock 1 r L emp%F k 4 2)
+               ∗ (⤉ isSpinlock N r L (counter N 2 5 r1 r2) k 4 2)
                ∗ live[k] (1/2)
-               ∗ ◇[k](3, 100)
-               ∗ (⤉ (counter_inv r1 r2 1))
+               ∗ ◇[k](3, 101)
                ∗ ➢(auexa_w r1 0)
-               ∗ (⤉ ((D ↦ 0) -U-[w](0)-◇ (t2_write_inv 1)))
+               ∗ (⤉ ((D ↦ 0) -U-[w](0)-◇ (t2_write_inv N r2)))
             )
               -∗
-              syn_wpsim 2 tid ∅
-              (fun rs rt => (⤉(syn_term_cond 1 tid _ rs rt))%F)
+              syn_wpsim (1+N) tid ∅
+              (fun rs rt => (⤉(syn_term_cond N tid _ rs rt))%F)
               false false
               (fn2th Client03Spec.module "thread1" (tt ↑))
-              (fn2th Client03.module "thread1" (tt ↑)))%F, 2⟧.
+              (fn2th Client03.module "thread1" (tt ↑)))%F, 1+N⟧.
   Proof.
-    Local Opaque incr.
     iIntros. simpl. red_tl; iIntros (r). red_tl. iIntros (k). red_tl. iIntros (w). red_tl. iIntros (r1). red_tl. iIntros (r2).
     red_tl. simpl.
     rewrite red_syn_tgt_interp_as. rewrite red_syn_until_tpromise. rewrite red_syn_wpsim.
-    unfold counter_inv. rewrite red_syn_inv.
-    iIntros "(#MEM & TID & DUTY & #ISL & LIVE_k & PC_k & #CNT & CNTW_r1 & UNTIL)".
+    iIntros "(#MEM & TID & DUTY & #ISL & LIVE_k & PC_k & CNTW_r1 & UNTIL)".
     unfold fn2th. simpl. lred2r. rred2r.
     iApply (wpsim_yieldR with "[DUTY]").
     2:{ iSplitL "DUTY". iApply "DUTY". simpl. ss. }
     auto.
-    iIntros "DUTY FC". iModIntro. rred2r. iApply wpsim_tauR. rred2r.
+    iIntros "DUTY _". iModIntro. rred2r. iApply wpsim_tauR. rred2r.
     assert (exists j, 0 = j). eauto. des.
     replace 
       (ITree.iter
@@ -198,13 +290,37 @@ Section SPEC.
     assert (100 = J). subst. ss.
     iEval (rewrite H0) in "PC_k". iEval (rewrite H) in "CNTW_r1".
     assert (LT : j <= 100). subst. lia.
-    clear H0 H. iClear "FC".
-    iRevert "MEM ISL CNT TID LIVE_k PC_k CNTW_r1 UNTIL DUTY". iStopProof.
+    clear H0 H.
+    iRevert "MEM ISL TID LIVE_k PC_k CNTW_r1 UNTIL DUTY". iStopProof.
     revert j HeqJ LT. induction J; cycle 1.
-    { i. iIntros "_ #MEM #ISL #CNT TID LIVE_k PC_k CNTW_r1 UNTIL DUTY".
+    { i. iIntros "_ #MEM #ISL TID LIVE_k PC_k CNTW_r1 UNTIL DUTY".
       iEval (rewrite unfold_iter_eq). rred2r.
       destruct (Nat.eq_dec j 100).
       { exfalso. lia. }
+      rred2.
+      iPoseProof (pc_split _ _ 1 (S J) with "PC_k") as "[PC_k1 PC_k]".
+      iApply (Client03_incr_spec with "[DUTY LIVE_k PC_k1 CNTW_r1] [TID UNTIL PC_k]").
+      ss.
+      { red_tl. simpl. iSplitR. rewrite red_syn_tgt_interp_as. eauto. iFrame.
+        simpl. do 3 (iSplitR; [iApply pcs_nil |]). iSplit. eauto. auto.
+      }
+      iEval red_tl. iIntros (_) "(DUTY & LIVE_k & CNTW_r1)". rred2r.
+      iApply (wpsim_yieldR with "[DUTY]").
+      2:{ iSplitL "DUTY". iApply "DUTY". simpl. ss. }
+      auto.
+      iIntros "DUTY _". iModIntro. rred2r. iApply wpsim_tauR. rred2r.
+      iApply wpsim_tauR.
+      specialize (IHJ (j+1)).
+      iPoseProof (IHJ with "[] MEM ISL TID LIVE_k PC_k CNTW_r1 UNTIL DUTY") as "IH".
+      { lia. }
+      { lia. }
+      { auto. }
+      iApply "IH".
+    }
+    { i. iIntros "_ #MEM #ISL TID LIVE_k PC_k CNTW_r1 UNTIL DUTY".
+      iEval (rewrite unfold_iter_eq). rred2r.
+      destruct (Nat.eq_dec j 100).
+      2:{ exfalso. lia. }
       rred2.
 
       TODO
@@ -212,17 +328,6 @@ Section SPEC.
 
 
     
-    iEval (rewrite unfold_iter_eq). rred2r.
-    iApply (SCMem_store_fun_spec _ _ tid n n with "[] [DUTY FC]").
-    auto. admit. admit.
-    iIntros (rv) "PT".
-    rred2r. iApply wpsim_tauR. rred2r. iEval (rewrite unfold_iter_eq). rred2r.
-    iApply (wpsim_yieldR with "[DUTY]"). 2: iFrame. auto.
-    iIntros "DUTY _". iModIntro. rred2r. iApply wpsim_tauR. rred2r.
-    iApply (Spinlock_lock_spec with "[DUTY PT FC] []").
-    ss. ss.
-    { red_tl. iFrame. instantiate (6:=⌜1 = 1⌝%F). admit. }
-    iIntros (_). red_tl. iIntros "[%u S]". iEval (red_tl) in "S".
 
   Admitted.
 
